extraction/theories/ExtractionCorrectness.v
@@ -67,17 +67,20 @@ Proof.
     + depelim ev.
 Qed.
 
-Theorem extract_correct (Σ : P.global_env_ext) kn ui ind c ui' (wfΣ : wf_ext Σ) exΣ :
+Theorem extract_correct
+        (Σ : P.global_env_ext) (wfΣ : wf_ext Σ)
+        kn ui ind c ui' ignored exΣ :
   axiom_free Σ ->
   welltyped Σ [] (P.tConst kn ui) ->
   Σ p⊢ P.tConst kn ui ▷ P.tConstruct ind c ui' ->
   (isErasable Σ [] (P.tConstruct ind c ui') -> False) ->
+  (forall k, ignored k = false) ->
   extract_pcuic_env
-    (pcuic_params check_masks_args)
-    Σ (wf_ext_wf_squash wfΣ) [kn] (fun _ => false) = Ok exΣ ->
+    (pcuic_args extract_within_coq)
+    Σ (wf_ext_wf_squash wfΣ) [kn] ignored = Ok exΣ ->
   trans_env exΣ e⊢ E.tConst kn ▷ E.tConstruct ind c.
 Proof.
-  intros ax [T wt] ev not_erasable ex.
+  intros ax [T wt] ev not_erasable no_ignores ex.
   cbn in *.
   destruct erase_global_decls_deps_recursive as [Σex|] eqn:er; cbn in *; [|congruence].
   destruct env_closed eqn:closed; cbn in *; [|congruence].
@@ -115,3 +118,26 @@ Proof.
   - cbn.
     now rewrite no_mask.
 Qed.
+
+Print Assumptions extract_correct.
+
+(* There are some assumptions of which almost all are in MetaCoq.
+   There are three assumptions in the list from this project.
+
+   1. metacoq_cofix_erasure_is_admitted, used in from MetaCoqErasureCorrectnessStrong.v.
+      This admission comes from the original MetaCoq development from which the proof was
+      adapted to be stronger. Since we do not extract cofixes this does not matter much.
+
+   2. hnf_completion, which is used in flag_of_type. These cases require a completion
+      statement about the hnf function from MetaCoq, saying that this function actually
+      reduces to head normal from. MetaCoq does not yet include a completeness statement
+      about hnf (but it is planned), so for now we defer those proofs.
+
+   3. assume_env_wellformed, which is used to assume that the environments we extract are
+      wellformed. MetaCoq's safe checker does not run from within Coq, so we cannot type
+      check the environments. However, our environments are unquoted directly from Coq's
+      kernel where they are already welltyped, so this is justified (and the same assumption
+      is used in MetaCoq when they run their erasure).
+
+   The rest of the assumptions are normal MetaCoq assumptions
+   (which are justified in Coq Coq Correct!) and todos left in the MetaCoq development. *)
